generalized the downward-closed sets used for computation trees into their own type of downward-closed sets; defined fixed-points on downward-closed sets, but still need to prove that the generalization to function types works...

theories/TraceMonad.v
@@ -78,12 +78,129 @@ Proof.
 Defined.
 
 Instance LR_Prop : LR Prop :=
-  { lr_leq := Basics.impl }.
+  { lr_leq P1 P2 := P1 -> P2 }.
 Proof.
   constructor.
   - intros P H; assumption.
   - intros P1 P2 P3 impl12 impl23 pf; apply impl23; apply impl12; assumption.
 Defined.
+
+
+(***
+ *** Downward Closed Sets
+ ***)
+
+Record DownSet A `{LR A} : Type :=
+  { inDownSet : A -> Prop;
+    downSetClosed :
+      forall a1 a2, lr_leq a2 a1 -> inDownSet a1 -> inDownSet a2 }.
+
+Arguments inDownSet {A _} _ _.
+Arguments downSetClosed {A _} _.
+
+Instance LR_DownSet A `{LR A} : LR (DownSet A) :=
+  {| lr_leq ds1 ds2 := lr_leq (inDownSet ds1) (inDownSet ds2) |}.
+Proof.
+  constructor.
+  - intro. reflexivity.
+  - intros ds1 ds2 ds3; transitivity (inDownSet ds2); assumption.
+Defined.
+
+Program Definition downClose {A} `{LR A} (a:A) : DownSet A :=
+  {| inDownSet a' := lr_leq a' a |}.
+Next Obligation.
+  etransitivity; eassumption.
+Defined.
+
+Instance Proper_downClose A `{LR A} :
+  Proper (lr_leq ==> lr_leq) (downClose (A:=A)).
+Proof.
+  intros a1 a2 R12 a'; simpl; intro in_a'. etransitivity; eassumption.
+Qed.
+
+Program Definition bindDownSet {A B} `{LR A} `{LR B}
+           (dsA: DownSet A) (f: A -> DownSet B) : DownSet B :=
+  {| inDownSet := fun b => exists a, inDownSet dsA a /\ inDownSet (f a) b;
+     downSetClosed := _ |}.
+Next Obligation.
+  exists H2; split; try assumption.
+  apply (downSetClosed _ _ _ H1 H4).
+Defined.
+
+Instance Proper_bindDownSet A B `{LR A} `{LR B} :
+  Proper (lr_leq ==> lr_leq ==> lr_leq) (bindDownSet (A:=A) (B:=B)).
+Proof.
+  intros ds1 ds2 Rds f1 f2 Rf b; simpl; intro in_b.
+  destruct in_b as [ a [in_ds1 in_f1]].
+  exists a; split.
+  - apply Rds; assumption.
+  - apply Rf; assumption.
+Qed.
+
+Definition mapDownSet {A B} `{LR A} `{LR B} (f:A -> B) dsA : DownSet B :=
+  bindDownSet dsA (fun a => downClose (f a)).
+
+Definition lambdaDownSet {A B} `{LR A} `{LR B}
+           (f: A -> DownSet B) : DownSet (A -> DownSet B) := downClose f.
+
+Definition applyDownSet {A B} `{LR A} `{LR B}
+           (dsF: DownSet (A -> DownSet B)) (a:A) : DownSet B :=
+  bindDownSet dsF (fun f => f a).
+
+
+Lemma downSetBeta {A B} `{LR A} `{LR B} (f: A -> DownSet B) :
+  applyDownSet (lambdaDownSet f) =lr= f.
+Proof.
+  split; simpl; intros.
+  - destruct H1 as [g [Rgf in_ga]]. apply Rgf; assumption.
+  - exists f; split; intros; assumption.
+Qed.
+
+(* NOTE: the reverse direction does not hold, because, e.g., dsF could be the
+union of (downClose f) and (downClose g) where f and g have distinct sets as
+their outputs for a, but (lambdaDownSet (applyDownSet dsF)) would have the union
+of these sets as the output for a. *)
+Lemma downSetEta {A B} `{LR A} `{LR B} (dsF : DownSet (A -> DownSet B)) :
+  dsF <lr= lambdaDownSet (applyDownSet dsF).
+Proof.
+  simpl; intros. exists a. split; assumption.
+Qed.
+
+
+Program Definition fixDownSet {A} `{LR A} (f: DownSet A -> DownSet A) : DownSet A :=
+  {| inDownSet a :=
+       forall ds, f ds <lr= ds -> inDownSet ds a
+  |}.
+Next Obligation.
+  apply (downSetClosed _ _ _ H0). apply H1. apply H2.
+Defined.
+
+Lemma fixDownSetUnfold {A} `{LR A} (f: DownSet A -> DownSet A)
+      (prp: Proper (lr_leq ==> lr_leq) f) :
+  (fixDownSet (A:=A) f) =lr= f (fixDownSet f).
+Proof.
+  assert (f (fixDownSet f) <lr= fixDownSet f).
+  - intros a in_a ds ds_f_closed.
+    assert (f (fixDownSet f) <lr= ds).
+    + etransitivity; try eassumption. apply prp.
+      intros a' in_a'. apply in_a'. assumption.
+    + apply H0; assumption.
+  - split; [ | apply H0 ].
+    simpl; intros; apply (H1 _ (prp _ _ H0)).
+Qed.
+
+(* FIXME: come up with a better name for this! *)
+Definition fixDownSetFun {A B} `{LR A} `{LR B}
+           (f: (A -> DownSet B) -> (A -> DownSet B))
+  : A -> DownSet B :=
+  applyDownSet (fixDownSet (fun ds => lambdaDownSet (f (applyDownSet ds)))).
+
+Lemma fixDownSetFunUnfold {A B} `{LR A} `{LR B}
+      (f: (A -> DownSet B) -> (A -> DownSet B))
+      (prp: Proper (lr_leq ==> lr_leq) f) :
+  fixDownSetFun f =lr= f (fixDownSetFun f).
+
+FIXME HERE NOW: prove this!
 
 
 (***
@@ -130,55 +247,19 @@ Instance LR_FinCompTree {St A} : LR (FinCompTree St A) :=
 
 
 (***
- *** Computation Trees
+ *** Transition Monads
  ***)
 
-(* A "computation tree" is a prefix-closed set of finite trees *)
-Record CompTree St A : Type :=
-  { ctIn : FinCompTree St A -> Prop;
-    ctClosed : forall tree1 tree2,
-        extendsFCT tree2 tree1 -> ctIn tree1 -> ctIn tree2 }.
-
-Arguments ctIn {St A} _.
-Arguments ctClosed {St A} _.
-
-Instance LR_CompTree St A : LR (CompTree St A) :=
-  { lr_leq := fun tree1 tree2 => lr_leq (ctIn tree1) (ctIn tree2) }.
-Proof.
-  constructor.
-  - intro. reflexivity.
-  - intros tree1 tree2 tree3; transitivity (ctIn tree2); assumption.
-Qed.
-
-
-Program Definition downCloseTree {St A} tree : CompTree St A :=
-  {|
-    ctIn := fun tree' => lr_leq tree' tree;
-  |}.
-Next Obligation.
-  etransitivity; eassumption.
-Defined.
-
-Instance Proper_downCloseTree St A :
-  Proper (lr_leq ==> lr_leq) (@downCloseTree St A).
-Proof.
-  admit. (* FIXME HERE *)
-Admitted.
-
-
-(***
- *** Stateful Monads
- ***)
-
-Class MonadStateOps M St : Type :=
+Class MonadTransOps M St : Type :=
   {
     returnM : forall {A}, A -> M A;
     bindM : forall {A B}, M A -> (A -> M B) -> M B;
     getM : M St;
     putM : St -> M unit;
+    yieldM : M unit;
   }.
 
-Class MonadState M St `{MonadStateOps M St} : Type :=
+Class MonadTrans M St `{MonadTransOps M St} : Type :=
   {
     Monad_LR {A} :> LR (M A);
 
@@ -192,7 +273,7 @@ Class MonadState M St `{MonadStateOps M St} : Type :=
     monad_assoc {A B C} m (f: A -> M B) (g: B -> M C) :
       bindM (bindM m f) g =lr= bindM m (fun x => bindM (f x) g);
 
-    (* FIXME HERE: write the monad laws! *)
+    (* FIXME HERE: write the state monad laws! *)
   }.
 
 
@@ -217,15 +298,16 @@ Proof.
   admit. (* FIXME HERE *)
 Admitted.
 
-Instance MonadStateOps_FinTraceMonad St : MonadStateOps (FinTraceMonad St) St :=
+Instance MonadTransOps_FinTraceMonad St : MonadTransOps (FinTraceMonad St) St :=
   {|
-    returnM := fun A a s => TreeLeaf s a;
-    bindM := fun A B m f s => bindFinTree (m s) f;
+    returnM A a := fun s => TreeLeaf s a;
+    bindM A B m f := fun s => bindFinTree (m s) f;
     getM := fun s => TreeLeaf s s;
-    putM := fun s _ => TreeLeaf s tt
+    putM s := fun _ => TreeLeaf s tt;
+    yieldM := fun s => TreeNode s (fun s => TreeLeaf s tt)
   |}.
 
-Instance MonadState_FinTraceMonad St : MonadState (FinTraceMonad St) St.
+Instance MonadTrans_FinTraceMonad St : MonadTrans (FinTraceMonad St) St.
 Proof.
   admit. (* FIXME HERE *)
 Admitted.
@@ -235,33 +317,66 @@ Admitted.
  *** The Trace Monad
  ***)
 
+Definition CompTree St A := DownSet (FinCompTree St A).
+
+Program Definition TreeNodeF {St A} (s:St)
+           (step: St -> CompTree St A) : CompTree St A :=
+  {| inDownSet fct :=
+         exists step',
+           fct <lr= TreeNode s step' /\
+           forall s', inDownSet (step s) (step' s')
+  |}.
+Next Obligation.
+  destruct a1; simpl in H1; try contradiction;
+    destruct a2; simpl in H; try contradiction; simpl.
+  - exists H0; split; [ apply I | assumption ].
+  - exists H0; split; [ apply I | assumption ].
+  - destruct H as [ eq10 R10 ]; destruct H1 as [ eq0_ R0_ ].
+    exists H0; split; [ split | ]; intros.
+    + etransitivity; eassumption.
+    + etransitivity; [ apply R10 | apply R0_ ].
+    + apply H2.
+Defined.
+
 Definition TraceMonad St A := St -> CompTree St A.
 
-Definition downCloseM {St A} (m: FinTraceMonad St A) : TraceMonad St A :=
-  fun s => downCloseTree (m s).
-
-
-FIXME HERE NOW: write bindTree!
-
-Program Definition bindTree {St A B} (tree: CompTree St A)
+Fixpoint bindFinTreeTM {St A B} (fct: FinCompTree St A)
         (f: A -> TraceMonad St B) : CompTree St B :=
-  {| ctIn := fun ftreeB =>
-               exists 
+  match fct with
+  | TreeStuck => downClose TreeStuck
+  | TreeLeaf s a => f a s
+  | TreeNode s step =>
+    TreeNodeF s (fun s' => bindFinTreeTM (step s') f)
+  end.
 
-Instance MonadStateOps_TraceMonad St : MonadStateOps (TraceMonad St) St :=
+Instance MonadTransOps_TraceMonad St : MonadTransOps (TraceMonad St) St :=
   {|
-    returnM := fun A a => downCloseM (returnM a);
-    bindM :=
-      fun A B m f =>
-        
+    returnM A a s := downClose (returnM a s);
+    bindM A B m f s :=
+      bindDownSet (m s) (fun fct => bindFinTreeTM fct f);
+    getM s := downClose (getM s);
+    putM s s' := downClose (putM s s');
+    yieldM s := downClose (yieldM s);
+  |}.
+
+Instance MonadTrans_TraceMonad St : MonadTrans (TraceMonad St) St.
+Proof.
+  admit.
+Admitted.
 
 
-Definition approxTM {St A} `{LR A}
-           (m: TraceMonad St A) (ftm: FinTraceMonad St A) : Prop :=
-  forall s, ctIn (m s) (ftm s).
+(***
+ *** Computation Traces in the Trace Monad
+ ***)
 
 Definition stepsTo1 {St A} `{LR A} : relation (St * TraceMonad St A) :=
   fun stm1 stm2 =>
-    forall ftm,
-      approxTM (snd stm2) ftm
-      <-> ctIn ((snd stm1) (fst stm1)) (TreeNode (fst stm2) ftm).
+    TreeNodeF (fst stm2) (snd stm2) <lr= (snd stm1) (fst stm1).
+
+Definition stepsTo {St A} `{LR A} := clos_trans _ (stepsTo1 (St:=St) (A:=A)).
+
+Definition evalsTo1 {St A} `{LR A} (stm : St * TraceMonad St A) (res : St * A) :=
+  inDownSet ((snd stm) (fst stm)) (TreeLeaf (fst res) (snd res)).
+
+Definition evalsTo {St A} `{LR A} (stm : St * TraceMonad St A) (res : St * A) :=
+  exists2 stm', stepsTo stm stm' & evalsTo1 stm' res.
